Freigen/CompM/Examples/Nondet/Defs.lean
@@ -8,8 +8,7 @@ inductive Eff : Type
 | rand
 | print
 
-def Spec : Eff.Spec where
-  tag := Eff
+instance : Eff.Spec Eff where
   input
     | .rand => Unit
     | .print => ℤ
@@ -22,22 +21,21 @@ def Spec : Eff.Spec where
 
 end Nondet
 
-abbrev Nondet α := CompM Nondet.Spec α
+abbrev Nondet α := CompM (Eff.Tau ⊕ Nondet.Eff) α
 
 namespace Nondet
 
-def rand : Nondet ℤ := CompM.op (E := Spec) Eff.rand () nofun
-def print (z : ℤ) : Nondet Unit := CompM.op (E := Spec) Eff.print z nofun
+def rand : Nondet ℤ := CompM.op (E := Eff.Tau ⊕ Eff) (Sum.inr Eff.rand) () nofun
+def print (z : ℤ) : Nondet Unit := CompM.op (E := Eff.Tau ⊕ Eff) (Sum.inr Eff.print) z nofun
 
 def approxWith {α} (entropy : ℕ → ℤ) (t : Nondet α) (n: Nat): List ℤ :=
   go (entropy, 0) n ((t.run pure).approx n) where
-  go : (ℕ → ℤ) × ℕ → (n : Nat) → IxPoly.M.Approx (Eff.Step Spec) n α → List ℤ := fun entropy n approx => match n, approx with
+  go : (ℕ → ℤ) × ℕ → (n : Nat) → IxPoly.M.Approx (Eff.Step $ Eff.Tau ⊕ Eff) n α → List ℤ := fun entropy n approx => match n, approx with
    | 0, IxPoly.M.Approx.zero _ => []
    | n+1, IxPoly.M.Approx._succ _ _ p k => match p with
      | .ret _ => []
-     | .tau => go entropy n (k ())
-     | .op Eff.rand () => go (entropy.1, entropy.2 + 1) n (k $ .inl (entropy.1 entropy.2))
-     | .op Eff.print z => z :: go entropy n (k $ .inl ())
-     | .fail => []
+     | .op (Sum.inr Eff.rand) () => go (entropy.1, entropy.2 + 1) n (k $ .inl (entropy.1 entropy.2))
+     | .op (Sum.inr Eff.print) z => z :: go entropy n (k $ .inl ())
+     | .op (Sum.inl _) _ => go entropy n (k $ .inl ())
 
 end Freigen.CompM.Examples.Nondet
