Freigen/Eff.lean
@@ -2,66 +2,162 @@ import Freigen.IxPoly.Basic
 
 namespace Freigen.Eff
 
-structure Spec where
-  tag : Type u
+class Spec (tag : Type u) where
   input : tag → Type v
   output : tag → Type v
   blockTag : tag → Type u
   blockInputs : (t : tag) → blockTag t → Type v
   blockOutputs : (t : tag) → blockTag t → Type v
 
-inductive NodeTag (E : Spec) : Type _ → Type _ where
-| ret {R} : R → NodeTag E R
-| tau {R} : NodeTag E R
-| fail {R} : NodeTag E R
-| op {R} (e : E.tag) : E.input e → NodeTag E R
+inductive NodeTag (T : Type u) [s: Spec T] : Type _ → Type _ where
+| ret {R} : R → NodeTag T R
+| op {R} (t : T) : s.input t → NodeTag T R
 
-def NodeTag.fields {i} {E : Spec}: NodeTag E i → Type _
+def NodeTag.fields {i} {T : Type u} [s : Spec T]: NodeTag T i → Type _
 | ret _ => PEmpty
-| tau => PUnit
-| fail => PEmpty
-| op e _ => E.output e ⊕ ((t : E.blockTag e) × E.blockInputs e t)
+| op e _ => s.output e ⊕ ((t : s.blockTag e) × s.blockInputs e t)
 
-def NodeTag.elem {E : Spec.{u, v}} {α : Type v} :
-    (t : NodeTag E α) → (p : t.fields) → Type v
+def NodeTag.elem {T : Type u} [s : Spec T] {α : Type v} :
+    (t : NodeTag T α) → (p : t.fields) → Type v
 | ret _, x => nomatch x
-| fail, x => nomatch x
-| tau, PUnit.unit => α
 | op _ _, Sum.inl _ => α
-| op e _, Sum.inr ⟨o, _⟩ => E.blockOutputs e o
+| op e _, Sum.inr ⟨o, _⟩ => s.blockOutputs e o
 
-def Empty : Spec where
-  tag := PEmpty
+instance : Spec PEmpty where
   input := nofun
   output := nofun
   blockTag := nofun
   blockInputs := nofun
   blockOutputs := nofun
 
-def Step (E : Spec.{u, v}) : IxPoly.Endo (Type v) where
-  Tag := fun α => NodeTag E α
+instance sumInst {T₁ T₂ : Type u} [Spec T₁] [Spec T₂] : Spec (T₁ ⊕ T₂) where
+  input := fun
+    | Sum.inl t => Spec.input t
+    | Sum.inr t => Spec.input t
+  output := fun
+    | Sum.inl t => Spec.output t
+    | Sum.inr t => Spec.output t
+  blockTag := fun
+    | Sum.inl t => Spec.blockTag t
+    | Sum.inr t => Spec.blockTag t
+  blockInputs := fun
+    | Sum.inl t => Spec.blockInputs t
+    | Sum.inr t => Spec.blockInputs t
+  blockOutputs := fun
+    | Sum.inl t => Spec.blockOutputs t
+    | Sum.inr t => Spec.blockOutputs t
+
+class inductive Has : (a: Type u) → [Spec a] → (b: Type u) → [Spec b] → Type _ where
+| here {α : Type u} [s : Spec α] : Has α α
+| inl {α β γ : Type u} [Spec α] [Spec β] [Spec γ] : Has α β → Has α (β ⊕ γ)
+| inr {α β γ : Type u} [Spec α] [Spec β] [Spec γ] : Has α γ → Has α (β ⊕ γ)
+
+instance [Spec α] : Has α α := Has.here
+instance [Spec α] [Spec β] [Spec γ] [r: Has α β] : Has α (β ⊕ γ) := Has.inl r
+instance [Spec α] [Spec β] [Spec γ] [r: Has α γ] : Has α (β ⊕ γ) := Has.inr r
+
+def Has.mk {α β} [Spec α] [Spec β] [r: Has α β] : α → β
+| a => match r with
+  | Has.here => a
+  | Has.inl r => Sum.inl (Has.mk a)
+  | Has.inr r => Sum.inr (Has.mk a)
+
+def Has.out {α β} [Spec α] [Spec β] [r: Has α β] : β → Option α
+| b => match r, b with
+  | Has.here, b => some b
+  | Has.inl _, Sum.inl a => Has.out a
+  | Has.inl _, Sum.inr _ => none
+  | Has.inr _, Sum.inl _ => none
+  | Has.inr _, Sum.inr a => Has.out a
+
+def Step (T : Type u) [Spec T] : IxPoly.Endo (Type v) where
+  Tag := fun α => NodeTag T α
   Field := fun _=> NodeTag.fields
   Elem := fun _ => NodeTag.elem
 
+structure Tau : Type u
+instance : Spec Tau where
+  input := fun _ => PUnit
+  output := fun _ => PUnit
+  blockTag := fun _ => PEmpty
+  blockInputs := fun _ => nofun
+  blockOutputs := fun _ => nofun
+
 namespace Step
 
-def ret {E α Y} (x : α) : Step E Y α := ⟨.ret x, fun a => PEmpty.elim a⟩
-def tau {E α Y} (x : Y α) : Step E Y α :=
-  ⟨.tau, fun
-    | PUnit.unit => x⟩
-def fail {E α Y} : Step E Y α := ⟨.fail, fun a => PEmpty.elim a⟩
-def op {E α Y} (e : E.tag) (inp : E.input e)
-    (blocks : (t : E.blockTag e) → E.blockInputs e t → Y (E.blockOutputs e t))
-    (k : (o : E.output e) → Y α) : Step E Y α :=
+def ret {E α Y} [Spec E] (x : α) : Step E Y α := ⟨.ret x, fun a => PEmpty.elim a⟩
+def op {E α Y} [s: Spec E] (e : E) (inp : s.input e)
+    (blocks : (t : s.blockTag e) → s.blockInputs e t → Y (s.blockOutputs e t))
+    (k : (o : s.output e) → Y α) : Step E Y α :=
   ⟨.op e inp, fun
     | Sum.inl o => k o
     | Sum.inr ⟨t, i⟩ => blocks t i
   ⟩
 
-protected def casesOn {E Y} { motive : (α : Type _) → Step E Y α → Sort* } {α} (x : Step E Y α)
+def Has.liftInput {E F} [s: Spec E] [s' : Spec F] (h : Has F E) (e : F) (inp : s'.input e) : s.input (Has.mk e) :=
+  match h with
+  | Has.here => inp
+  | Has.inl r => liftInput r e inp
+  | Has.inr r => liftInput r e inp
+
+def Has.lowerBlockTag {E F} [s: Spec E] [s' : Spec F] [h : Has F E] {e : F} (t : s.blockTag (Has.mk e)) : s'.blockTag e :=
+  match h with
+  | Has.here => t
+  | Has.inl r => lowerBlockTag (h:=r) t
+  | Has.inr r => lowerBlockTag (h:=r) t
+
+def Has.lowerBlockInput {E F} [s: Spec E] [s' : Spec F] [h : Has F E]: {e : F} → (t : s.blockTag (Has.mk e)) →
+    (i : s.blockInputs (Has.mk e) t) → s'.blockInputs e (lowerBlockTag t) :=
+  match h with
+  | Has.here => fun _ i => i
+  | Has.inl r => fun t i => lowerBlockInput (h:=r) t i
+  | Has.inr r => fun t i => lowerBlockInput (h:=r) t i
+
+def Has.liftBlockOutput
+    {E F} {Y : Type v → Type w}
+    [s : Spec E] [s' : Spec F] [h : Has F E] :
+    {e : F} →
+    (t : s.blockTag (Has.mk e)) →
+    Y (s'.blockOutputs e (Has.lowerBlockTag t)) →
+    Y (s.blockOutputs (Has.mk e) t) := match h with
+  | Has.here => fun _ x => x
+  | Has.inl r => fun t x => liftBlockOutput (h:=r) t x
+  | Has.inr r => fun t x => liftBlockOutput (h:=r) t x
+
+def Has.lowerOutput
+    {E F} [s : Spec E] [s' : Spec F] [h : Has F E]
+    {e : F} (o : s.output (Has.mk e)) :
+    s'.output e := match h with
+  | Has.here => o
+  | Has.inl r => lowerOutput (h:=r) o
+  | Has.inr r => lowerOutput (h:=r) o
+
+def Has.op {E F α Y} [s: Spec E] [s': Spec F] [h: Has F E] (e : F) (inp : s'.input e)
+    (blocks : (t : s'.blockTag e) → s'.blockInputs e t → Y (s'.blockOutputs e t))
+    (k : (o : s'.output e) → Y α) : Step E Y α :=
+  Step.op (Has.mk e)
+     (Has.liftInput h e inp)
+     (fun t i => Has.liftBlockOutput t $ blocks (Has.lowerBlockTag t) (Has.lowerBlockInput t i))
+     (fun o => k (Has.lowerOutput o))
+
+ theorem Has.liftBlockOutput_naturality
+      {E F} {Y : Type v → Type w} {Z : Type v → Type z}
+      [s : Spec E] [s' : Spec F] [h : Has F E]
+      (f : (α : Type v) → Y α → Z α) {e : F}
+      (t : s.blockTag (Has.mk e))
+      (x : Y (s'.blockOutputs e (Has.lowerBlockTag t))) :
+      f _ (Has.liftBlockOutput (Y := Y) t x) =
+        Has.liftBlockOutput (Y := Z) t (f _ x) := by
+    induction h with
+    | here => rfl
+    | inl r ih => exact ih t x
+    | inr r ih => exact ih t x
+
+def tau {E α Y} [Spec E] [Has Tau E] (x : Y α) : Step E Y α := Has.op Tau.mk () nofun (fun () => x)
+
+
+protected def casesOn {E Y} [Spec E] { motive : (α : Type _) → Step E Y α → Sort* } {α} (x : Step E Y α)
     (ret : ∀ {α} x, motive α (ret x))
-    (tau : ∀ {α} x, motive α (tau x))
-    (fail : ∀ {α}, motive α fail)
     (op : ∀ {α} e inp blocks k, motive α (op e inp blocks k)):
     motive α x := by
   rcases x with ⟨tag, fields⟩
@@ -71,16 +167,6 @@ protected def casesOn {E Y} { motive : (α : Type _) → Step E Y α → Sort* }
     simp only [Step.ret]
     congr 2
     ext a; cases a
-  | tau =>
-    convert tau (fields PUnit.unit)
-    · rfl
-    · simp only [Step.tau]
-      congr
-  | fail =>
-    convert fail
-    simp only [Step.fail]
-    congr 2
-    ext a; cases a
   | op e inp =>
     convert op e inp (fun t i => fields (.inr ⟨t, i⟩)) (fun o => fields (.inl o))
     simp only [Step.op]
@@ -88,38 +174,60 @@ protected def casesOn {E Y} { motive : (α : Type _) → Step E Y α → Sort* }
     ext a; cases a <;> rfl
 
 @[simp]
-theorem map_ret {E} {Y Z : Type _ → Type _} {f : (α : Type _) → Y α → Z α} {α : Type _} {x : α}:
+theorem map_ret {E} [Spec E] {Y Z : Type _ → Type _} {f : (α : Type _) → Y α → Z α} {α : Type _} {x : α}:
     IxPoly.map (F := Step E) f α (Step.ret x) = Step.ret x := by
   simp only [IxPoly.map, ret]
   congr 1
   ext a; cases a
 
-@[simp]
-theorem map_tau {E} {Y Z : Type _ → Type _} {f : (α : Type _) → Y α → Z α} {α : Type _} {x : Y α}:
-    IxPoly.map (F := Step E) f α (Step.tau x) = Step.tau (f α x) := by
-  simp only [IxPoly.map, tau]
-  congr 1
+
+
+-- @[simp]
+-- theorem map_fail {E} {Y Z : Type _ → Type _} {f : (α : Type _) → Y α → Z α} {α : Type _}:
+--     IxPoly.map (F := Step E) f α (Step.fail) = Step.fail := by
+--   simp only [IxPoly.map, fail]
+--   congr 1
+--   ext a; cases a
 
 @[simp]
-theorem map_fail {E} {Y Z : Type _ → Type _} {f : (α : Type _) → Y α → Z α} {α : Type _}:
-    IxPoly.map (F := Step E) f α (Step.fail) = Step.fail := by
-  simp only [IxPoly.map, fail]
-  congr 1
-  ext a; cases a
-
-@[simp]
-theorem map_op {E} {Y Z : Type _ → Type _} {f : (α : Type _) → Y α → Z α} {α : Type _}
-    {e : E.tag} {inp : E.input e}
-    {blocks : (t : E.blockTag e) → E.blockInputs e t → Y (E.blockOutputs e t)}
-    {k : (o : E.output e) → Y α}:
+theorem map_op {E} [h: Spec E] {Y Z : Type _ → Type _} {f : (α : Type _) → Y α → Z α} {α : Type _}
+    {e : E} {inp : h.input e}
+    {blocks : (t : h.blockTag e) → h.blockInputs e t → Y (h.blockOutputs e t)}
+    {k : (o : h.output e) → Y α}:
     IxPoly.map (F := Step E) f α (Step.op e inp blocks k) =
       Step.op e inp (fun t i => f _ (blocks t i)) (fun o => f _ (k o)) := by
   simp only [IxPoly.map, op]
   congr 1
   ext a; cases a <;> rfl
 
-theorem tau_def {E} {Y : Type _ → Type _} {α : Type _} {x : Y α}:
-    Step.tau (E := E) x = ⟨.tau, fun _ => x⟩ := by rfl
+  @[simp]
+  theorem map_hasOp
+      {E F} [Spec E] [Spec F] [Has F E]
+      {Y Z : Type _ → Type _}
+      (f : (α : Type _) → Y α → Z α) {α}
+      (e : F) (inp : Spec.input e)
+      (blocks :
+        (t : Spec.blockTag e) →
+        Spec.blockInputs e t →
+        Y (Spec.blockOutputs e t))
+      (k : Spec.output e → Y α) :
+      IxPoly.map (F := Step E) f α (Has.op e inp blocks k) =
+        Has.op e inp
+          (fun t i => f _ (blocks t i))
+          (fun o => f _ (k o)) := by
+    unfold Has.op
+    rw [map_op]
+    congr 1
+    funext t i
+    apply Has.liftBlockOutput_naturality
+
+@[simp]
+theorem map_tau {E} [Spec E] [Has Tau E] {Y Z : Type _ → Type _} {f : (α : Type _) → Y α → Z α} {α : Type _} {x : Y α}:
+    IxPoly.map (F := Step E) f α (Step.tau x) = Step.tau (f α x) := by
+  simp only [tau, map_hasOp]
+  congr 1
+  ext a
+  cases a
 
 end Step
 
