Freigen/Circuit/Defs.lean
@@ -1,0 +1,49 @@
+import Freigen.CompM.Basic
+import Freigen.Eff
+
+namespace Freigen.Circuit
+
+inductive Eff : Type _
+| assert
+| hint (tp : Type)
+
+def Eff.input : Eff → Type _
+| .assert => Bool
+| .hint _ => Unit
+
+def Eff.output : Eff → Type
+| .assert => Unit
+| .hint tp => tp
+
+def Eff.blockTag : Eff → Type _
+| .assert => PEmpty
+| .hint _ => PUnit
+
+def Eff.blockInputs : (t : Eff) → Eff.blockTag t → Type
+| assert => nofun
+| hint _ => fun _ => Unit
+
+def Eff.blockOutputs : (t : Eff) → Eff.blockTag t → Type
+| assert => nofun
+| hint tp => fun _ => tp
+
+instance : Freigen.Eff.Spec Eff where
+  input := Eff.input
+  output := Eff.output
+  blockTag := Eff.blockTag
+  blockInputs := Eff.blockInputs
+  blockOutputs := Eff.blockOutputs
+
+end Circuit
+
+def Circuit : Type → Type _ := CompM (Eff.Tau ⊕ Circuit.Eff)
+
+namespace Circuit
+
+def assert (b : Bool) : Circuit Unit :=
+  CompM.op (E := Eff.Tau ⊕ Circuit.Eff) (.inr Eff.assert) b nofun
+
+def hint {α : Type} : Circuit α → Circuit α := fun hint =>
+  CompM.op (E := Eff.Tau ⊕ Circuit.Eff) (.inr (Eff.hint α)) () fun _ _ => hint
+
+end Freigen.Circuit
