Freigen/Free.lean
@@ -4,21 +4,21 @@ import Freigen.Eff
 
 namespace Freigen
 
-def wBind {α β} {E} (a : IxPoly.W (Eff.Step E) α) (f : α → IxPoly.W (Eff.Step E) β): IxPoly.W (Eff.Step E) β := match a with
+variable {E : Type u} [eS: Eff.Spec E] {α β : Type}
+
+def wBind {α β} (a : IxPoly.W (Eff.Step E) α) (f : α → IxPoly.W (Eff.Step E) β): IxPoly.W (Eff.Step E) β := match a with
   | IxPoly.W.mk i p g => match p with
     | .ret a => f a
-    | .tau => IxPoly.W.roll (Eff.Step.tau $ wBind (g ()) f)
-    | .fail => IxPoly.W.roll (Eff.Step.fail)
     | .op e inp => IxPoly.W.mk (F := Eff.Step E) _ (Eff.NodeTag.op e inp) (fun
       | .inl a => wBind (g (.inl a)) f
       | .inr b => g (.inr b)
     )
 
-instance {E} : Monad (IxPoly.W (Eff.Step E)) where
+instance : Monad (IxPoly.W (Eff.Step E)) where
   pure a := IxPoly.W.roll (Eff.Step.ret a)
   bind x f := wBind x f
 
-instance {E} : LawfulMonad (IxPoly.W (Eff.Step E)) := LawfulMonad.mk' _
+instance : LawfulMonad (IxPoly.W (Eff.Step E)) := LawfulMonad.mk' _
   (by
     intro _ x
     change wBind x (fun a => IxPoly.W.roll (Eff.Step.ret a)) = x
@@ -28,15 +28,6 @@ instance {E} : LawfulMonad (IxPoly.W (Eff.Step E)) := LawfulMonad.mk' _
       · simp [wBind, IxPoly.W.roll, Eff.Step.ret]
         ext a
         cases a
-      · have := ih ()
-        simp only [wBind, IxPoly.W.roll, Eff.Step.tau]
-        simp only [IxPoly.W.roll] at this
-        simp only [IxPoly.W.mk.injEq, heq_eq_eq, true_and]
-        ext x; cases x
-        simp only
-        exact this
-      · simp [wBind, IxPoly.W.roll, Eff.Step.fail]
-        ext x; cases x;
       · simp only [wBind]
         congr
         ext x
@@ -52,12 +43,6 @@ instance {E} : LawfulMonad (IxPoly.W (Eff.Step E)) := LawfulMonad.mk' _
     | mk i p g ih =>
       cases p
       · rfl
-      · simp only [Bind.bind, wBind, Eff.Step.tau, IxPoly.W.roll]
-        congr 1
-        ext x; cases x
-        simp only
-        apply ih
-      · simp only [Bind.bind, wBind, Eff.Step.fail, IxPoly.W.roll]
       · simp only [Bind.bind, wBind]
         congr
         ext x; cases x
@@ -66,11 +51,12 @@ instance {E} : LawfulMonad (IxPoly.W (Eff.Step E)) := LawfulMonad.mk' _
         · rfl
   )
 
-def Free (E : Eff.Spec) (α : Type) : Type _ := ExactCodensity (IxPoly.W (Eff.Step E)) α
+def Free (E : Type u) [Eff.Spec E] (α : Type) : Type _ :=
+    ExactCodensity (IxPoly.W (Eff.Step E)) α
 
-instance {E} : Monad (Free E) :=
+instance : Monad (Free E) :=
   inferInstanceAs (Monad (ExactCodensity (IxPoly.W (Eff.Step E))))
-instance {E} : LawfulMonad (Free E) :=
+instance : LawfulMonad (Free E) :=
   inferInstanceAs (LawfulMonad (ExactCodensity (IxPoly.W (Eff.Step E))))
 
 end Freigen
